wip

ProducerConsumerMath.dfy
@@ -2,21 +2,18 @@ include "CivlizedMathPrelude.dfy"
 include "../../fl/spec/refinement.s.dfy"
 include "../../fl/util/simulation.i.dfy"
 include "../../fl/util/refinement/AnnotatedBehavior.i.dfy"
+include "../../fl/util/refinement/RefinementConvolution.i.dfy"
+include "../../util/collections/seqs.i.dfy"
 
 module ProducerConsumerConfig {
     datatype Config = Config
 }
 
-module ProducerConsumerAction {
-    datatype Action = InputAction | OutputAction
-}
-
-
 module ProducerConsumer {
     import opened util_option_s
     import opened Prelude
-    import opened GeneralRefinementModule
-    import opened ProducerConsumerAction
+    import opened AnnotatedBehaviorModule
+    import opened ProducerConsumerConfig
 
     datatype SharedState = SharedState(buffer: Option<int>)
 
@@ -33,6 +30,8 @@ module ProducerConsumer {
                          | ConsumerThread(consumerpc: ConsumerPC, consumerstate: ConsumerState)
 
     type State = TotalState<SharedState, ThreadState>
+
+    datatype Action = ForkAction(forked_tid: Tid) | NopAction | InputAction | ProduceAction | ConsumeAction | OutputAction
 
 
     function ProducerInitSet(): iset<ThreadState>
@@ -78,79 +77,86 @@ module ProducerConsumer {
         && s'.shared.buffer.None?
     }
 
-    predicate ProducerNext(tid: Tid, s: State, s': State)
+    predicate ProducerNext(tid: Tid, s: State, s': State, a: Action)
         requires tid in s.locals && s.locals[tid].Some? && s.locals[tid].v.ProducerThread? && s.locals.Keys <= s'.locals.Keys
     {
         match s.locals[tid].v.producerpc
             case ProducerPC0 => 
                 && s'.locals[tid].Some?
                 && s'.locals[tid].v.ProducerThread?
+                && a.InputAction?
                 && Input(tid, s, s', s'.locals[tid].v.producerstate.x)
                 && s'.locals[tid].v.producerpc == ProducerPC1
             case ProducerPC1 => 
                 && s'.locals[tid].Some?
                 && s'.locals[tid].v.ProducerThread?
+                && a.ProduceAction?
                 && Produce(tid, s, s', s.locals[tid].v.producerstate.x)
                 && s'.locals[tid].v.producerpc == ProducerPC0
     }
 
-    predicate ConsumerNext(tid: Tid, s: State, s': State)
+    predicate ConsumerNext(tid: Tid, s: State, s': State, a: Action)
         requires tid in s.locals && s.locals[tid].Some? && s.locals[tid].v.ConsumerThread? && s.locals.Keys <= s'.locals.Keys
     {
         match s.locals[tid].v.consumerpc
             case ConsumerPC0 => 
                 && s'.locals[tid].Some?
                 && s'.locals[tid].v.ConsumerThread?
+                && a.ConsumeAction?
                 && Consume(tid, s, s', s'.locals[tid].v.consumerstate.x)
                 && s'.locals[tid].v.consumerpc == ConsumerPC1
             case ConsumerPC1 => 
                 && s'.locals[tid].Some?
                 && s'.locals[tid].v.ConsumerThread?
+                && a.OutputAction?
                 && Output(tid, s, s', s.locals[tid].v.consumerstate.x)
                 && s'.locals[tid].v.consumerpc == ConsumerPC0
     }
 
-    predicate MainNext(tid: Tid, s: State, s': State)
+    predicate MainNext(tid: Tid, s: State, s': State, a: Action)
         requires tid in s.locals && s.locals[tid].Some? && s.locals[tid].v.MainThread? && s.locals.Keys <= s'.locals.Keys
     {
         match s.locals[tid].v.mainpc
             case MainPC0 => 
                 && s'.locals[tid].Some?
                 && s'.locals[tid].v.MainThread?
-                && (exists tid' :: Fork(tid, s, s', ProducerInitSet(), tid'))
+                && a.ForkAction?
+                && Fork(tid, s, s', ProducerInitSet(), a.forked_tid)
                 && s'.locals[tid].v.mainpc == MainPC1
             case MainPC1 => 
                 && s'.locals[tid].Some?
                 && s'.locals[tid].v.MainThread?
-                && (exists tid' :: Fork(tid, s, s', ConsumerInitSet(), tid'))
+                && a.ForkAction?
+                && Fork(tid, s, s', ProducerInitSet(), a.forked_tid)
                 && s'.locals[tid].v.mainpc == MainPC2
             case MainPC2 => 
                 && s'.locals[tid].Some?
                 && s'.locals[tid].v.MainThread?
+                && a.NopAction?
                 && Nop(tid, s, s')
                 && s'.locals[tid].v.mainpc == MainPC2
     }
 
-    predicate ThreadNext(tid: Tid, s: State, s': State)
+    predicate ThreadNext(tid: Tid, s: State, s': State, a: Action)
     {
         && tid in s.locals
         && s.locals[tid].Some?
         && s.locals.Keys <= s'.locals.Keys
         && (forall tid' :: tid' != tid && tid' in s.locals ==> s'.locals[tid'] == s.locals[tid'])
         && match s.locals[tid].v
-            case MainThread(_,_) => MainNext(tid, s, s')
-            case ProducerThread(_, _) => ProducerNext(tid, s, s')
-            case ConsumerThread(_, _) => ConsumerNext(tid, s, s')
+            case MainThread(_,_) => MainNext(tid, s, s', a)
+            case ProducerThread(_, _) => ProducerNext(tid, s, s', a)
+            case ConsumerThread(_, _) => ConsumerNext(tid, s, s', a)
     }
 
-    predicate Next(s: State, s': State)
+    predicate Next(s: State, s': State, a: Action)
     {
-        exists tid :: ThreadNext(tid, s, s')
+        exists tid :: ThreadNext(tid, s, s', a)
     }
 
-    function GetSpec(): Spec<State>
+    function GetSpec(c: Config): AnnotatedBehaviorSpec<Config, State, Action>
     {
-        Spec(iset s | Init(s), iset s, s' | Next(s, s') :: StatePair(s, s'))
+        AnnotatedBehaviorSpec(c, iset s | Init(s), iset s, s', a | Next(s, s', a) :: ActionTuple(s, s', a))
     }
 }
 
@@ -159,7 +165,6 @@ module ProducerConsumerSpec {
     import opened GeneralRefinementModule
     import opened ProducerConsumerConfig
     import opened AnnotatedBehaviorModule
-    import opened ProducerConsumerAction
 
     datatype SharedState = SharedState
 
@@ -169,6 +174,8 @@ module ProducerConsumerSpec {
     datatype ThreadState = MainThread(mainpc: MainPC, mainstate: MainState)
 
     type State = TotalState<SharedState, ThreadState>
+
+    datatype Action = InputAction | OutputAction
 
     function MainInitSet(): iset<ThreadState>
     {
@@ -223,55 +230,14 @@ module ProducerConsumerSpec {
         exists tid :: ThreadNext(tid, s, s', a)
     }
 
-    function GetSpec(c: Config): AnnotatedBehaviorSpec<Config, State, Action>
+    function GetNext(): iset<ActionTuple<State, Action>>
     {
-        AnnotatedBehaviorSpec(c, iset s | Init(s),
-            iset s, s', a | Next(s, s', a) :: ActionTuple(s, s', a))
-    }
-}
-
-module AnnotatedHighSpec {
-    import opened util_option_s
-    import opened Prelude
-    import opened AnnotatedBehaviorModule
-    import opened ProducerConsumerConfig
-
-    datatype State = State(log: seq<Event>, pending: Option<int>)
-
-    predicate Init(s: State) 
-    {
-        && s.log == []
-        && s.pending.None?
-    }
-
-    datatype Action = InputAction(x: int) | OutputAction(x: int)
-
-    predicate Input(s: State, s': State, a: Action)
-    {
-        && a.InputAction?
-        && s.pending.None?
-        && s'.pending == Some(a.x)
-        && s'.log == s.log + [InputEvent(a.x)]
-    }
-
-    predicate Output(s: State, s': State, a: Action)
-    {
-        && a.OutputAction?
-        && a.x == s.pending.v
-        && s.pending.Some?
-        && s'.pending.None?
-        && s'.log == s.log + [OutputEvent(s.pending.v)]
-    }
-
-    predicate Next(s: State, s': State, a: Action)
-    {
-        || Input(s, s', a)
-        || Output(s, s', a)
+        iset s, s', a | Next(s, s', a) :: ActionTuple(s, s', a)
     }
 
     function GetSpec(c: Config): AnnotatedBehaviorSpec<Config, State, Action>
     {
-        AnnotatedBehaviorSpec(c, iset s | Init(s), iset s, s', a | Next(s, s', a) :: ActionTuple(s, s', a))
+        AnnotatedBehaviorSpec(c, iset s | Init(s), GetNext())
     }
 }
 
@@ -315,16 +281,19 @@ module HighSpec {
     }
 }
 
-module PCHighRefinementRelation {
-    import opened GeneralRefinementModule
-    import ProducerConsumerSpec
-    import HighSpec
-
+module PrefixModule {
     predicate IsPrefix<A>(small: seq<A>, big: seq<A>)
     {
         && |small| <= |big|
         && forall i :: 0 <= i < |small| ==> small[i] == big[i]
     }
+}
+
+module PCSpecHighRefinementRelation {
+    import opened GeneralRefinementModule
+    import opened PrefixModule
+    import ProducerConsumerSpec
+    import HighSpec
 
     function GetRelation(): RefinementRelation<ProducerConsumerSpec.State, HighSpec.State>
     {
@@ -332,41 +301,129 @@ module PCHighRefinementRelation {
     }
 }
 
-module PCSpecRefinesAnnotatedHighSpec {
+module PCPCSpecRefinementRelation {
+    import opened GeneralRefinementModule
+    import opened PrefixModule
+    import ProducerConsumer
+    import ProducerConsumerSpec
+
+    function GetRelation(): RefinementRelation<ProducerConsumer.State, ProducerConsumerSpec.State>
+    {
+        iset l: ProducerConsumer.State, h: ProducerConsumerSpec.State | IsPrefix(l.external, h.external) :: RefinementPair(l, h)
+    }
+}
+
+module PCHighRefinementRelation {
+    import opened GeneralRefinementModule
+    import opened PrefixModule
+    import ProducerConsumer
+    import HighSpec
+
+    function GetRelation(): RefinementRelation<ProducerConsumer.State, HighSpec.State>
+    {
+        iset l: ProducerConsumer.State, h: HighSpec.State | IsPrefix(l.external, h.log) :: RefinementPair(l, h)
+    }
+}
+
+
+module PCRefinesPCSpec {
     import opened util_option_s
     import opened Prelude
     import opened GeneralRefinementModule
-    import opened SimulationModule
+    import opened AnnotatedBehaviorModule
     import opened ProducerConsumerConfig
+    import opened RefinementConvolutionModule
+    import ProducerConsumer
     import ProducerConsumerSpec
-    import AnnotatedHighSpec
     import PCHighRefinementRelation
+    import PCSpecHighRefinementRelation
 
-    predicate SimulationRelation(l: ProducerConsumerSpec.State, h: AnnotatedHighSpec.State)
+    predicate SimulationRelation(l: ProducerConsumer.State, h: ProducerConsumerSpec.State)
     {
         true
     }
 
-    function GetSimulationRelation():
-        RefinementRelation<ProducerConsumerSpec.State, AnnotatedHighSpec.State>
+    lemma lemma_PCBehaviorToPCSpecBehavior(
+        lb: AnnotatedBehavior<Config, ProducerConsumer.State, ProducerConsumer.Action>
+        ) returns (
+        hb: AnnotatedBehavior<Config, ProducerConsumerSpec.State, ProducerConsumerSpec.Action>
+        )
+        requires AnnotatedBehaviorSatisfiesSpec(lb, ProducerConsumer.GetSpec(lb.config))
+        ensures lb.config == hb.config
+        ensures AnnotatedBehaviorSatisfiesSpec(hb, ProducerConsumerSpec.GetSpec(hb.config))
+        ensures BehaviorRefinesWhatOtherBehaviorRefines(lb.states, hb.states, 
+            PCHighRefinementRelation.GetRelation(), 
+            PCSpecHighRefinementRelation.GetRelation())
     {
-        iset l, h| SimulationRelation(l, h) :: RefinementPair(l, h)
+        assume false;
+    }
+}
+
+module PCSpecRefinesHighSpec {
+    import opened util_option_s
+    import opened Prelude
+    import opened GeneralRefinementModule
+    import opened AnnotatedBehaviorModule
+    import opened ProducerConsumerConfig
+    import opened util_collections_seqs_i
+    import ProducerConsumerSpec
+    import HighSpec
+    import PCSpecHighRefinementRelation
+
+    predicate SimulationRelation(l: ProducerConsumerSpec.State, h: HighSpec.State)
+    {
+        && l.external == h.log
+        && exists main_tid :: 
+            && l.locals.Keys == {main_tid}
+            && l.locals[main_tid].Some?
+            && match l.locals[main_tid].v.mainpc
+                case MainPC0 => h.pending.None?
+                case MainPC1 => h.pending == Some(l.locals[main_tid].v.mainstate.x)
     }
 
-    lemma lemma_PCSpecRefinesHighSpec(c: Config)
-        ensures SpecRefinesSpec(ProducerConsumerSpec.GetSpec(), AnnotatedHighSpec.GetSpec(c),
-                                PCHighRefinementRelation.GetRelation())
-    {
-        var l_spec := ProducerConsumerSpec.GetSpec();
-        var h_spec := AnnotatedHighSpec.GetSpec(c);
-        var relation := PCHighRefinementRelation.GetRelation();
 
-        forall lb | BehaviorSatisfiesSpec(lb, l_spec)
-            ensures BehaviorRefinesSpec(lb, h_spec, relation)
+    lemma lemma_PCSpecBehaviorToHighBehavior(
+        lb: AnnotatedBehavior<Config, ProducerConsumerSpec.State, ProducerConsumerSpec.Action>
+        ) returns (
+        hb: seq<HighSpec.State>
+        )
+        requires AnnotatedBehaviorSatisfiesSpec(lb, ProducerConsumerSpec.GetSpec(lb.config))
+        ensures BehaviorSatisfiesSpec(hb, HighSpec.GetSpec())
+        ensures BehaviorRefinesBehavior(lb.states, hb, PCSpecHighRefinementRelation.GetRelation())
+    {
+        assert ProducerConsumerSpec.Init(lb.states[0]);
+        var hb0 := HighSpec.State([], None);
+        assert SimulationRelation(lb.states[0], hb0);
+        hb := [hb0];
+
+        while |hb| < |lb.states|
+            invariant 0 <= |hb| <= |lb.states|
+            invariant forall i :: 0 <= i < |hb| ==> SimulationRelation(lb.states[i], hb[i])
+            invariant BehaviorSatisfiesSpec(hb, HighSpec.GetSpec())
         {
-//            var sr := SimulationRequest(l_spec, h_spec, relation, GetSimulationRelation(), iset s | true);
-            var hb := [];
-            assert BehaviorRefinesBehavior(lb, hb, relation);
+            var i := |hb|-1;
+            var l, l', a := lb.states[i], lb.states[i+1], lb.trace[i];
+            var h := hb[i];
+            assert SimulationRelation(l, h);
+            assert ActionTuple(l, l', a) in ProducerConsumerSpec.GetNext();
+            var tid :| ProducerConsumerSpec.ThreadNext(tid, l, l', a);
+            assert l.locals.Keys == {tid};
+            var h': HighSpec.State;
+            match l.locals[tid].v.mainpc {
+                case MainPC0 => {
+                    var x := l'.locals[tid].v.mainstate.x;
+                    h' := HighSpec.State(h.log + [InputEvent(x)], Some(x));
+                }
+                case MainPC1 => {
+                    var x := l.locals[tid].v.mainstate.x;
+                    h' := HighSpec.State(h.log + [OutputEvent(x)], None);
+                }
+            }
+
+            hb := hb + [h'];
         }
+
+        var lh_map := ConvertMapToSeq(|hb|, map i | 0 <= i < |hb| :: RefinementRange(i, i));
+        assert BehaviorRefinesBehaviorUsingRefinementMap(lb.states, hb, PCSpecHighRefinementRelation.GetRelation(), lh_map);
     }
 }
